Replace subset variant of In by inductive variant

theories/Context.v
@@ -39,6 +39,7 @@ From MasterThesis Require Import
      Prelude.
 
 Local Set Implicit Arguments.
+Local Unset Equations Derive Equations.
 
 Declare Scope ctx_scope.
 Delimit Scope ctx_scope with ctx.
@@ -154,125 +155,47 @@ Module ctx.
     End WithUIP.
 
     Section In.
-      (* Set locally only for the definition of In. *)
-      Local Set Primitive Projections.
-
-       (* InCtx represents context containment proofs. This is essentially a
+       (* In represents context containment proofs. This is essentially a
           well-typed de Bruijn index, i.e. a de Bruijn index with a proof that it
-          resolves to the binding b. This record type is defined using primitive
-          projections to get eta-conversion definitionally. *)
-      Class In (b : B) (Γ : Ctx B) : Set :=
-        MkIn
-          { in_at: nat;
-            in_valid: nth_is Γ in_at b
-          }.
-
-      Global Arguments MkIn [_ _] _ _.
-      Global Arguments in_at [_ _] _.
-      Global Arguments in_valid [_ _] _.
-
-      Local Obligation Tactic := idtac.
-
-      Global Program Instance NoConfusionPackage_In {uip_B : UIP B} {b Γ} : NoConfusionPackage (In b Γ) :=
-         {| NoConfusion xIn yIn := NoConfusion (in_at xIn) (in_at yIn);
-            noConfusion xIn yIn (e : NoConfusion (in_at xIn) (in_at yIn)) :=
-              match noConfusion e in _ = y
-                return forall q, xIn = {| in_at := y; in_valid := q |}
-              with
-              | eq_refl => fun q => f_equal (MkIn _) (proof_irrelevance_nth_is _ _ (in_valid xIn) q)
-              end (in_valid yIn);
-            noConfusion_inv (xIn yIn : In b Γ) (e : xIn = yIn) :=
-              noConfusion_inv (f_equal (@in_at b Γ) e);
-         |}.
-      Next Obligation.
-        intros ? ? ? [m p] [n q] e. cbn [in_at] in *.
-        change (NoConfusion _ _) with (NoConfusion m n) in e.
-        destruct (noConfusion e) eqn:?. cbn.
-        destruct (proof_irrelevance_nth_is m b p q). cbn.
-        destruct m.
-        - destruct e. reflexivity.
-        - apply uip.
-      Qed.
-      Next Obligation.
-        intros ? ? ? [m p] [n q] e; intros.
-        destruct e.
-        destruct Γ; cbn in *. contradiction.
-        destruct m, n.
-        - destruct p. cbn. now rewrite EqDec.uip_refl_refl.
-        - destruct p. cbn. now rewrite EqDec.uip_refl_refl.
-        - cbn. rewrite proof_irrelevance_nth_is_refl. reflexivity.
-        - cbn. rewrite proof_irrelevance_nth_is_refl. reflexivity.
-      Qed.
+          resolves to the binding b.  *)
+      Inductive In (b : B) : Ctx B -> Set :=
+      | in_zero {Γ : Ctx B} : In b (snoc Γ b)
+      | in_succ {Γ : Ctx B} {b' : B} (bIn : In b Γ) : In b (snoc Γ b').
+      Existing Class In.
+      Global Arguments in_zero {b Γ}.
+      Derive Signature NoConfusion for In.
 
     End In.
 
-    (* Two proofs of context containment are equal of the deBruijn indices are equal *)
-    Definition In_eqb {Γ} {b1 b2 : B} (b1inΓ : In b1 Γ) (b2inΓ : In b2 Γ) : bool :=
-      Nat.eqb (in_at b1inΓ) (in_at b2inΓ).
+    (* (* Two proofs of context containment are equal of the deBruijn indices are equal *) *)
+    (* Definition In_eqb {Γ} {b1 b2 : B} (b1inΓ : In b1 Γ) (b2inΓ : In b2 Γ) : bool := *)
+    (*   Nat.eqb (in_at b1inΓ) (in_at b2inΓ). *)
 
-    Lemma In_eqb_spec `{UIP B} {Γ} {b1 b2 : B} (b1inΓ : In b1 Γ) (b2inΓ : In b2 Γ) :
-      reflect
-        (existT _ _ b1inΓ = existT _ _ b2inΓ :> sigT (fun b => In b Γ))
-        (In_eqb b1inΓ b2inΓ).
-    Proof.
-      destruct b1inΓ as [m p], b2inΓ as [n q]; cbn.
-      destruct (Nat.eqb_spec m n); constructor.
-      - subst. pose proof (nth_is_right_exact _ _ _ p q). subst.
-        f_equal. f_equal. apply proof_irrelevance_nth_is.
-      - intros e. depelim e. destruct n, m; cbn in H0; congruence.
-    Qed.
-
-    (* These are *constructors* for In. *)
-    Definition in_zero {b : B} {Γ : Ctx B} : In b (snoc Γ b) :=
-      @MkIn _ (snoc Γ b) 0 eq_refl.
-    Definition in_succ {b : B} {Γ : Ctx B} {b' : B} (bIn : In b Γ) :
-      In b (snoc Γ b') :=
-      @MkIn _ (snoc Γ b') (S (in_at bIn)) (in_valid bIn).
+    (* Lemma In_eqb_spec `{UIP B} {Γ} {b1 b2 : B} (b1inΓ : In b1 Γ) (b2inΓ : In b2 Γ) : *)
+    (*   reflect *)
+    (*     (existT _ _ b1inΓ = existT _ _ b2inΓ :> sigT (fun b => In b Γ)) *)
+    (*     (In_eqb b1inΓ b2inΓ). *)
+    (* Proof. *)
+    (*   destruct b1inΓ as [m p], b2inΓ as [n q]; cbn. *)
+    (*   destruct (Nat.eqb_spec m n); constructor. *)
+    (*   - subst. pose proof (nth_is_right_exact _ _ _ p q). subst. *)
+    (*     f_equal. f_equal. apply proof_irrelevance_nth_is. *)
+    (*   - intros e. depelim e. destruct n, m; cbn in H0; congruence. *)
+    (* Qed. *)
 
     Inductive NilView {b : B} (i : In b nil) : Set :=.
 
-    Definition nilView {b : B} (i : In b nil) : NilView i :=
-      match in_valid i with end.
+    Equations nilView {b : B} (i : In b nil) : NilView i :=.
 
     Inductive SnocView (Γ : Ctx B) {b' : B} : forall b, In b (snoc Γ b') -> Set :=
     | snocViewZero                  : SnocView in_zero
     | snocViewSucc {b} (i : In b Γ) : SnocView (in_succ i).
     Global Arguments snocViewZero {_ _}.
 
-    Definition snocView {Γ} {b b' : B} (i : In b (snoc Γ b')) :
+    Equations snocView {Γ} {b b' : B} (i : In b (snoc Γ b')) :
       @SnocView Γ b' b i :=
-      match in_at i as n return forall p, SnocView (MkIn n p)
-      with
-      | O   => fun p => match p with eq_refl => snocViewZero end
-      | S n => fun p => snocViewSucc (MkIn n p)
-      end (in_valid i).
-
-    (* Custom pattern matching in cases where the context was already refined
-       by a different match, i.e. on environments. *)
-    Definition in_case_nil {A : B -> Type} [b : B] (bIn : In b nil) : A b :=
-      match nilView bIn with end.
-    (* DEPRECATED *)
-    Definition in_case_snoc (D : B -> Type) (Γ : Ctx B) (b0 : B) (db0 : D b0)
-      (dΓ: forall b, In b Γ -> D b) (b : B) (bIn: In b (snoc Γ b0)) : D b :=
-      let (n, e) := bIn in
-      match n return nth_is (snoc Γ b0) n b -> D b with
-      | 0 => fun e => match e with eq_refl => db0 end
-      | S n => fun e => dΓ b (MkIn n e)
-      end e.
-
-    Inductive InView {b : B} : forall Γ, In b Γ -> Set :=
-    | inctxViewZero {Γ}                 : @InView b (snoc Γ b) in_zero
-    | inctxViewSucc {Γ b'} (i : In b Γ) : @InView b (snoc Γ b') (in_succ i).
-
-    Definition inView {b Γ} : forall bIn : In b Γ, InView bIn :=
-      match Γ with
-      | nil      => fun bIn => match nilView bIn with end
-      | snoc Γ b => fun bIn =>
-        match snocView bIn with
-        | snocViewZero   => inctxViewZero
-        | snocViewSucc i => inctxViewSucc i
-        end
-      end.
+    | in_zero   => snocViewZero
+    | in_succ i => snocViewSucc i.
 
     Fixpoint in_cat_left {b : B} {Γ : Ctx B} (Δ : Ctx B) (bIn : In b Γ) : In b (cat Γ Δ) :=
       match Δ with
@@ -280,20 +203,21 @@ Module ctx.
       | snoc Δ _ => in_succ (in_cat_left Δ bIn)
       end.
 
-    Fixpoint in_cat_right {b : B} {Γ : Ctx B} (Δ : Ctx B) : In b Δ -> In b (cat Γ Δ) :=
-      match Δ with
-      | nil      => fun bIn => match nilView bIn with end
-      | snoc _ _ =>
-        fun bIn =>
-          match snocView bIn with
-          | snocViewZero => in_zero
-          | snocViewSucc bIn => in_succ (in_cat_right bIn)
-          end
+    Fixpoint in_cat_right {b : B} {Γ : Ctx B} (Δ : Ctx B) (bIn : In b Δ) : In b (cat Γ Δ) :=
+      match bIn with
+      | in_zero   => in_zero
+      | in_succ i => in_succ (in_cat_right i)
       end.
 
     Inductive CatView {Γ Δ} {b : B} : In b (cat Γ Δ) -> Set :=
     | isCatLeft  (bIn : In b Γ) : CatView (in_cat_left Δ bIn)
     | isCatRight (bIn : In b Δ) : CatView (in_cat_right bIn).
+
+    Definition catView_nil {Γ b} (bIn : In b Γ) : @CatView Γ nil b bIn :=
+      @isCatLeft Γ nil b bIn.
+
+    Definition catView_zero {Γ Δ b} : @CatView Γ (snoc Δ b) b in_zero :=
+      @isCatRight Γ (snoc Δ b) b in_zero.
 
     Definition catView_succ {Γ Δ b b'} (bIn : In b (cat Γ Δ)) (bInV : CatView bIn) :
       @CatView Γ (snoc Δ b') b (in_succ bIn) :=
@@ -302,72 +226,10 @@ Module ctx.
       | isCatRight bIn => @isCatRight Γ (@snoc B Δ b') b (@in_succ b Δ b' bIn)
       end.
 
-    Fixpoint catView_index {Γ Δ} {b : B} {struct Δ} :
-      forall (n : nat) (p : nth_is (cat Γ Δ) n b),
-        @CatView Γ Δ b (@MkIn b (cat Γ Δ) n p) :=
-      match Δ with
-      | nil => fun n p => @isCatLeft Γ (@nil B) b (@MkIn b Γ n p)
-      | snoc Δ0 b0 =>
-        fun n =>
-          match n with
-          | 0 =>
-            fun p =>
-              match
-                p as e in (_ = y)
-                return (@CatView Γ (@snoc B Δ0 b0) y (@MkIn y (@snoc B (cat Γ Δ0) b0) 0 e))
-              with
-              | eq_refl => @isCatRight Γ (@snoc B Δ0 b0) b0 (@in_zero b0 Δ0)
-              end
-          | S n => fun p => catView_succ (catView_index n p)
-          end
-      end.
-
-    Definition catView {Γ Δ} {b : B} (bIn : In b (cat Γ Δ)) : CatView bIn :=
-      @catView_index Γ Δ b (@in_at _ _ bIn) (@in_valid _ _ bIn).
-
-    Definition In_rect (b : B)
-      (P : forall (Γ : Ctx B), In b Γ -> Type)
-      (fzero : forall (Γ : Ctx B), P (snoc Γ b) in_zero)
-      (fsucc : forall (Γ : Ctx B) (b0 : B) (bIn : In b Γ),
-          P Γ bIn -> P (snoc Γ b0) (in_succ bIn)) :
-      forall (Γ : Ctx B) (bIn : In b Γ), P Γ bIn.
-    Proof.
-      induction Γ; cbn.
-      - intro bIn. destruct (nilView bIn).
-      - intros bIn. destruct (snocView bIn).
-        + apply fzero.
-        + now apply fsucc.
-    Defined.
-    Global Arguments In_rect [_] _.
-
-    Definition In_ind (b : B)
-      (P : forall (Γ : Ctx B), In b Γ -> Prop)
-      (fzero : forall (Γ : Ctx B), P (snoc Γ b) in_zero)
-      (fsucc : forall (Γ : Ctx B) (b0 : B) (bIn : In b Γ),
-          P Γ bIn -> P (snoc Γ b0) (in_succ bIn)) :
-      forall (Γ : Ctx B) (bIn : In b Γ), P Γ bIn :=
-      In_rect P fzero fsucc.
-    Global Arguments In_ind [_] _.
-
-    (* Boolean equality of [nat]-fields in [In] implies equality of
-       the other field and the binding-index of [In] *)
-    Lemma in_at_exact {Γ : Ctx B} (b1 b2 : B)
-          (b1In : In b1 Γ) (b2In : In b2 Γ) :
-      @in_at _ _ b1In = @in_at _ _ b2In ->
-      b1 = b2 /\
-      (nth_is Γ (@in_at _ _ b1In) b1 = nth_is Γ (@in_at _ _ b2In) b2).
-    Proof.
-      intros.
-      assert (b1 = b2) as bindings_eq.
-      { generalize dependent b2.
-        induction b1In using In_ind; destruct b2In as [[|n] e];
-        intros; cbn in *; try congruence.
-        apply IHb1In with (MkIn n e).
-        cbn; congruence. }
-      split.
-      - exact bindings_eq.
-      - subst. f_equal. assumption.
-    Qed.
+    Equations catView {Γ} Δ {b : B} (bIn : In b (cat Γ Δ)) : CatView bIn :=
+    | nil      | bIn       => catView_nil bIn
+    | snoc Δ _ | in_zero   => catView_zero
+    | snoc Δ _ | in_succ i => catView_succ (catView Δ i).
 
     Section All.
 
@@ -385,8 +247,6 @@ Module ctx.
     End All.
 
   End WithBinding.
-  Arguments In_rect [B b] _ _ _ [_].
-  Arguments In_ind [B b] _ _ _ [_].
 
   Section WithAB.
     Context {A B : Set} (f : A -> B).
@@ -397,24 +257,12 @@ Module ctx.
       | snoc Γ a => snoc (map Γ) (f a)
       end.
 
-    (* This is proof relevant because it's used in the automatic translation
-       of program variables to logic variables. *)
-    Definition in_map {a : A} : forall Γ, In a Γ -> In (f a) (map Γ) :=
-      In_rect
-        (fun Γ _ => In (f a) (map Γ))
-        (fun Γ   => in_zero)
-        (fun Γ _ _ => in_succ).
-
   End WithAB.
 
   Module notations.
 
     Open Scope ctx_scope.
 
-    (* DEPRECATED *)
-    (* NB: ∶ ≠ : *)
-    (*    To typeset the next notation, use \: *)
-    Notation "x ∶ τ" := (MkB x τ) (only parsing) : ctx_scope.
     Notation "x :: τ" := (MkB x τ) (only parsing) : ctx_scope.
     Notation "N ∷ T" := (Binding N T) : type_scope.
     Notation "x ∷ t" := (MkB x t) : ctx_scope.
